module peano where

data ℕ : Set where
  zero : ℕ
  suc : ℕ → ℕ

{-# BUILTIN NATURAL ℕ #-}
import Relation.Binary.PropositionalEquality as Eq
open Eq using (_≡_; refl)
open Eq.≡-Reasoning using (begin_; _≡⟨⟩_; _∎)

_+_ : ℕ → ℕ → ℕ
infixl 6 _+_
zero + n     = n
suc m + n = suc (m + n)

_ : 2 + 3 ≡ 5
_ =
  begin
    2 + 3
  ≡⟨⟩    -- is shorthand for
    (suc (suc zero)) + (suc (suc (suc zero)))
  ≡⟨⟩    -- inductive case
    suc ((suc zero) + (suc (suc (suc zero))))
  ≡⟨⟩    -- inductive case
    suc (suc (zero + (suc (suc (suc zero)))))
  ≡⟨⟩    -- base case
    suc (suc (suc (suc (suc zero))))
  ≡⟨⟩    -- is longhand for
    5
  ∎

_ : 2 + 3 ≡ 5
_ =
  begin
    2 + 3
  ≡⟨⟩
    suc (1 + 3)
  ≡⟨⟩
    suc (suc (0 + 3))
  ≡⟨⟩
    suc (suc 3)
  ≡⟨⟩
    5
  ∎

_ : 2 + 3 ≡ 5
_ = refl

_ : 3 + 4 ≡ 7
_ =
  begin
    3 + 4
  ≡⟨⟩
    suc (2 + 4)
  ≡⟨⟩
    suc (suc (1 + 4))
  ≡⟨⟩
    suc (suc (suc (0 + 4)))
  ≡⟨⟩
    suc (suc (suc 4))
  ≡⟨⟩
    7
  ∎

_*_ : ℕ → ℕ → ℕ
infixl 7 _*_
zero * n = zero
(suc m) * n = n + (m * n)

_ =
  begin
    2 * 3
  ≡⟨⟩
    3 + (1 * 3)
  ≡⟨⟩
    3 + (3 + (0 * 3))
  ≡⟨⟩
    3 + (3 + 0)
  ≡⟨⟩
    6
  ∎

_ =
  begin
    3 * 4
  ≡⟨⟩
    4 + (4 + (1 * 4))
  ≡⟨⟩
    4 + (4 + (4 + (0 * 4)))
  ≡⟨⟩
    4 + (4 + (4 + 0))
  ≡⟨⟩
    12
  ∎

_^_ : ℕ → ℕ → ℕ
n ^ zero = 1
n ^ (suc m) = n * (n ^ m)

_ : 3 ^ 4 ≡ 81
_ =
  begin
    3 ^ 4
  ≡⟨⟩
    3 * (3 ^ 3)
  ≡⟨⟩
    3 * (3 * (3 ^ 2))
  ≡⟨⟩
    3 * (3 * (3 * (3 ^ 1)))
  ≡⟨⟩
    3 * (3 * (3 * (3 * (3 ^ 0))))
  ≡⟨⟩
    3 * (3 * (3 * (3 * 1)))
  ≡⟨⟩
    3 * (3 * (3 * 3))
  ≡⟨⟩
    81
  ∎

_∸_ : ℕ → ℕ → ℕ
infixl 6 _∸_
m ∸ zero = m
zero ∸ (suc n) = zero
(suc m) ∸ (suc n) = m ∸ n

_ =
  begin
    3 ∸ 2
  ≡⟨⟩
    2  ∸ 1
  ≡⟨⟩
    1 ∸ 0
  ≡⟨⟩
    1
  ∎

_ =
  begin
    2 ∸ 3
  ≡⟨⟩
    1 ∸ 2
  ≡⟨⟩
    0 ∸ 1
  ≡⟨⟩
    0
  ∎

_ =
  begin
    5 ∸ 3
  ≡⟨⟩
    4 ∸ 2
  ≡⟨⟩
    3 ∸ 1
  ≡⟨⟩
    2 ∸ 0
  ≡⟨⟩
    2
  ∎

_ =
  begin
    3 ∸ 5
  ≡⟨⟩
    2 ∸ 4
  ≡⟨⟩
    1 ∸ 3
  ≡⟨⟩
    0 ∸ 2
  ≡⟨⟩
    0
  ∎
